Clean up LList example

pulse/examples/steel/arraystructs/LList.fst
@@ -65,19 +65,42 @@ let elim_vpure
     (fun _ _ -> p)
     (fun m -> pure_interp p m; reveal_emp (); intro_emp m)
 
+val unreachable (#opened:inames) (#p:vprop) (#q:'a -> vprop) (r:'a -> prop)
+: SteelGhostF 'a opened p q (requires fun _ -> False) (ensures fun _ x _ -> r x)
+
+let unreachable (#opened:inames) (#p:vprop) (#q:'a -> vprop) (r:'a -> prop)
+: SteelGhostF 'a opened p q (requires fun _ -> False) (ensures fun _ x _ -> r x)
+= let x: 'a = FStar.IndefiniteDescription.indefinite_description_tot 'a (fun _ -> True) in
+  change_slprop_rel p (q x) (fun _ _ -> r x) (fun _ -> ());
+  x
+
 // ----------------------------------------
 
 open ListNode
 
-let cells = list (int & ptr node node)
+let cell = int & ptr node node
+let cells = list cell
+
+let hd_node (l: Ghost.erased cells): Ghost.erased (option node) =
+  match Ghost.reveal l with
+  | (value, next) :: _ -> some (mk_node (some value) (some next))
+  | [] -> none
+
+let pts_to_llist_tl (l:Ghost.erased cells)
+  (pts_to_llist:(
+    p:ptr node node -> 
+    l':Ghost.erased cells{List.length l' < List.length l} -> 
+    Tot vprop))
+: Tot vprop
+= match Ghost.reveal l with
+  | [] -> emp
+  | (value, next) :: tl -> next `pts_to_llist` tl
 
 let rec pts_to_llist (p:ptr node node) ([@@@smt_fallback] l:Ghost.erased cells)
 : Tot vprop (decreases (List.length l))
-= match Ghost.reveal l with
-  | [] -> vpure (p == nullptr)
-  | (value, next) :: tl ->
-    pts_to p node_pcm (mk_node (some value) (some next)) `star`
-    (next `pts_to_llist` Ghost.hide tl)
+= vpure (p == nullptr <==> Ghost.reveal l == []) `star`
+  pts_to_or_null p node_pcm (hd_node l) `star`
+  pts_to_llist_tl l pts_to_llist
 
 // TODO: should be something like:
 // pts_to_or_null p node_pcm (match l with [] -> one _ | (value, next) :: tl -> mk_node ...) `star`
@@ -88,48 +111,118 @@ let rec pts_to_llist (p:ptr node node) ([@@@smt_fallback] l:Ghost.erased cells)
 // end
 // TODO pts_to_or_null take option
 
-let pts_to_llist_nil_eq p
-: Lemma ((p `pts_to_llist` []) == vpure (p == nullptr))
-  [SMTPat (p `pts_to_llist` [])]
-= ()
+let unfold_pts_to_llist (#opened:inames) (p:ptr node node) (l:Ghost.erased cells)
+: SteelGhost unit opened
+    (p `pts_to_llist` l)
+    (fun _ -> 
+      pts_to_or_null p node_pcm (hd_node l) `star`
+      pts_to_llist_tl l pts_to_llist)
+    (requires fun _ -> True)
+    (ensures fun _ _ _ -> p == nullptr <==> Ghost.reveal l == [])
+= change_equal_slprop
+    (p `pts_to_llist` l)
+    (vpure (p == nullptr <==> Ghost.reveal l == []) `star`
+     pts_to_or_null p node_pcm (hd_node l) `star`
+     pts_to_llist_tl l pts_to_llist);
+  elim_vpure _
 
-let pts_to_llist_cons_eq (p:ptr node node) (value:int) (next:ptr node node) (tl:cells)
-: Lemma ((p `pts_to_llist` Ghost.hide ((value, next) :: tl)) == 
-    pts_to p node_pcm (mk_node (some value) (some next)) `star`
-    (next `pts_to_llist` Ghost.hide tl))
-= ()
-
-val intro_llist_nil : unit -> SteelT unit emp (fun _ -> nullptr `pts_to_llist` [])
-
-let intro_llist_nil () =
-  intro_vpure (nullptr #node #node == nullptr);
-  pts_to_llist_nil_eq nullptr;
-  change_equal_slprop _ (nullptr `pts_to_llist` [])
-  
-val intro_llist_cons
-  (#opened:inames) (p: ptr node node)
-  (value: int) (next: ptr node node)
-  (tl: cells)
-: SteelGhostT unit opened
-    ((pts_to p node_pcm (mk_node (some value) (some next))) `star` (next `pts_to_llist` tl))
-    (fun _ -> p `pts_to_llist` ((value, next)::tl))
-  
-let intro_llist_cons p' value next tl = change_equal_slprop _ _
-
-val elim_llist_cons
-  (#opened:inames) (p: ptr node node)
-  (value: int) (next: ptr node node) (tl: cells)
-: SteelGhostT unit opened
-    (p `pts_to_llist` ((value, next)::tl))
-    (fun _ ->
-      (pts_to p node_pcm (mk_node (some value) (some next))) `star`
-      (next `pts_to_llist` tl))
-
-let elim_llist_cons p value next tl =
+let fold_pts_to_llist (#opened:inames) (p:ptr node node) (l:Ghost.erased cells)
+: SteelGhost unit opened
+    (pts_to_or_null p node_pcm (hd_node l) `star`
+     pts_to_llist_tl l pts_to_llist)
+    (fun _ -> p `pts_to_llist` l)
+    (requires fun _ -> p == nullptr <==> Ghost.reveal l == [])
+    (ensures fun _ _ _ -> True)
+= intro_vpure (p == nullptr <==> Ghost.reveal l == []);
   change_equal_slprop
-    (p `pts_to_llist` ((value, next)::tl)) // TODO why can't these be inferred?
-    ((pts_to p node_pcm (mk_node (some value) (some next))) `star`
-     (next `pts_to_llist` tl))
+    (vpure (p == nullptr <==> Ghost.reveal l == []) `star`
+     pts_to_or_null p node_pcm (hd_node l) `star`
+     pts_to_llist_tl l pts_to_llist)
+    (p `pts_to_llist` l)
+
+let intro_pts_to_llist_nil #opened p
+: SteelGhost unit opened 
+    emp
+    (fun _ -> p `pts_to_llist` Ghost.hide [])
+    (requires fun _ -> p == nullptr)
+    (ensures fun _ _ _ -> True)
+= intro_vpure (p == nullptr <==> Ghost.reveal (Ghost.hide ([] #cell)) == []);
+  intro_pts_to_or_null_nullptr node_pcm;
+  change_equal_slprop
+    (vpure (p == nullptr <==> Ghost.reveal (Ghost.hide ([] #cell)) == []) `star`
+     pts_to_or_null (nullptr #node) node_pcm none `star` emp)
+    (p `pts_to_llist` Ghost.hide [])
+
+let elim_pts_to_llist_nil #opened p
+: SteelGhost unit opened 
+    (p `pts_to_llist` Ghost.hide [])
+    (fun _ -> emp)
+    (requires fun _ -> True)
+    (ensures fun _ _ _ -> p == nullptr)
+= change_equal_slprop
+    (p `pts_to_llist` Ghost.hide [])
+    (vpure (p == nullptr <==> Ghost.reveal (Ghost.hide ([] #cell)) == []) `star`
+     pts_to_or_null p node_pcm none `star` emp);
+  elim_vpure (p == nullptr <==> Ghost.reveal (Ghost.hide ([] #cell)) == []);
+  elim_pts_to_or_null_nullptr p
+
+let intro_pts_to_llist_cons #opened p value_next value next (l: Ghost.erased cells)
+: SteelGhost unit opened 
+    (pts_to p node_pcm value_next `star` (next `pts_to_llist` l))
+    (fun _ -> p `pts_to_llist` ((value, next) :: Ghost.reveal l))
+    (requires fun _ -> value_next == mk_node (some value) (some next))
+    (ensures fun _ _ _ -> p =!= nullptr)
+= change_equal_slprop
+    (pts_to p node_pcm value_next)
+    (pts_to p node_pcm (mk_node (some value) (some next)));
+  pts_to_nonnull p; assert (p =!= nullptr);
+  let l': Ghost.erased cells = Ghost.hide ((value, next) :: Ghost.reveal l) in
+  intro_vpure (p == nullptr <==> Ghost.reveal l' == []);
+  assert (hd_node l' == some (mk_node (some value) (some next)));
+  intro_pts_to_or_null p;
+  change_equal_slprop (next `pts_to_llist` l) (pts_to_llist_tl l' pts_to_llist);
+  change_equal_slprop
+    (vpure (p == nullptr <==> Ghost.reveal l' == []) `star`
+     pts_to_or_null p node_pcm (hd_node l') `star`
+     pts_to_llist_tl l' pts_to_llist)
+    (p `pts_to_llist` _)
+
+[@@erasable]
+noeq type elim_pts_to_llist_cons_res = {
+  value: int;
+  next: ptr node node;
+  tl: cells;
+}
+
+let elim_pts_to_llist_cons #opened p (l: Ghost.erased cells)
+: SteelGhost elim_pts_to_llist_cons_res opened 
+    (p `pts_to_llist` l)
+    (fun res ->
+      pts_to p node_pcm (mk_node (some res.value) (some res.next)) `star`
+      (res.next `pts_to_llist` res.tl))
+    (requires fun _ -> p =!= nullptr)
+    (ensures fun _ res _ -> Ghost.reveal l == (res.value, res.next) :: res.tl)
+= change_equal_slprop (p `pts_to_llist` l)
+    (vpure (p == nullptr <==> Ghost.reveal l == []) `star`
+     pts_to_or_null p node_pcm (hd_node l) `star`
+     pts_to_llist_tl l pts_to_llist);
+  elim_vpure (p == nullptr <==> Ghost.reveal l == []);
+  match Ghost.reveal l with
+  | [] -> unreachable (fun res -> Ghost.reveal l == (res.value, res.next) :: res.tl)
+  | (value, next) :: tl ->
+    assert (hd_node l == some (mk_node (some value) (some next)));
+    let w = elim_pts_to_or_null p in
+    assert (w == mk_node (some value) (some next));
+    change_equal_slprop (pts_to_llist_tl l pts_to_llist) (next `pts_to_llist` tl);
+    {value; next; tl}
+
+let ptr a = ptr a a
+
+let intro_llist_nil ()
+: SteelT (ptr node) emp (fun p -> p `pts_to_llist` [])
+= let p = nullptr in
+  intro_pts_to_llist_nil p;
+  return p
 
 let rec values (l:cells) : GTot (list int) =
   match l with
@@ -138,34 +231,26 @@ let rec values (l:cells) : GTot (list int) =
 
 #set-options "--ide_id_info_off"
 
-val push (p:ptr node node) (l:Ghost.erased cells) (value:int)
-: Steel (ptr node node & Ghost.erased cells)
+val push (p:ptr node) (l:Ghost.erased cells) (value:int)
+: Steel (ptr node & _)
     (p `pts_to_llist` l)
     (fun (p', l') -> p' `pts_to_llist` l')
     (requires fun _ -> True)
     (ensures fun _ (_, l') _ -> values l' == value :: values l)
 
 let push p l value =
-  let cell: int & ptr node node = (value, p) in
-  let r = ref_alloc node_pcm (mk_node_tot (Some value) (Some p)) in
+  let cell: int & ptr node = (value, p) in
+  let value_next: node = mk_node_tot (Some value) (Some p) in
+  let r = ref_alloc node_pcm value_next in
   let q = intro_pts_to r in
-  intro_llist_cons q value p l;
+  intro_pts_to_llist_cons q value_next value p l;
   return (q, Ghost.hide (cell :: l))
   
 let cells_set_hd x (l: cells) = match l with
   | [] -> []
   | (_, next) :: l' -> (x, next) :: l'
 
-val exfalso (#opened:inames) (p:vprop) (q:'a -> vprop) (r:'a -> prop)
-: SteelGhostF 'a opened p q (requires fun _ -> False) (ensures fun _ x _ -> r x)
-
-let exfalso (#opened:inames) (p:vprop) (q:'a -> vprop) (r:'a -> prop)
-: SteelGhostF 'a opened p q (requires fun _ -> False) (ensures fun _ x _ -> r x)
-= let x: 'a = FStar.IndefiniteDescription.indefinite_description_tot 'a (fun _ -> True) in
-  change_slprop_rel p (q x) (fun _ _ -> r x) (fun _ -> ());
-  x
-
-val pts_to_llist_nullptr (#opened:inames) (p:ptr node node) (l:Ghost.erased cells)
+val pts_to_llist_nullptr (#opened:inames) (p:ptr node) (l:Ghost.erased cells)
 : SteelGhost unit opened
     (p `pts_to_llist` l) 
     (fun _ -> p `pts_to_llist` l)
@@ -173,75 +258,88 @@ val pts_to_llist_nullptr (#opened:inames) (p:ptr node node) (l:Ghost.erased cell
     (ensures fun _ _ _ -> Ghost.reveal l == [])
 
 let pts_to_llist_nullptr p l =
-  match Ghost.reveal l with
-  | [] -> change_equal_slprop (p `pts_to_llist` l) (p `pts_to_llist` l) // TODO why can't just put ()
-  | (value, next) :: tl ->
-    change_equal_slprop (p `pts_to_llist` l) (p `pts_to_llist` ((value, next) :: tl));
-    let r = elim_llist_cons p value next tl in
-    pts_to_nonnull p;
-    assert (p =!= nullptr);
-    assert (p == nullptr);
-    exfalso _ _ (fun _ -> Ghost.reveal l == [])
+  unfold_pts_to_llist p l;
+  assert (Ghost.reveal l == []);
+  fold_pts_to_llist p l
 
-[@@erasable]
-noeq type pts_to_llist_res = {
-  value: int;
-  next: ptr node node;
-  tl: cells;
-}
+(* Currently z3 is going through the lemma
+      refine value /\ refine next ==> refine (mk_node value next)
+   plus the fact that for our PCMs, ~ refine one.
+   If change refine predicate/drop the side condition ~ refine one, will 
+   need to expose the proper lemmas about mk_node in ListNode.fsti
+*)
+let nontrivial_fact_about_mk_node value next
+: Lemma (Ghost.reveal (mk_node (some value) (some next)) =!= one node_pcm)
+= ()
 
-val pts_to_llist_some (#opened:inames) (p:ptr node node) (l:Ghost.erased cells)
-: SteelGhost pts_to_llist_res opened
-    (p `pts_to_llist` l) 
-    (fun res -> p `pts_to_llist` ((res.value, res.next) :: res.tl))
-    (requires fun _ -> p =!= nullptr)
-    (ensures fun _ res _ -> Ghost.reveal l == ((res.value, res.next) :: res.tl))
+assume val intro_pts_to_llist_cons' : #opened:inames ->
+      p: ptr node ->
+      value: int ->
+      next: ptr node ->
+      l: Ghost.erased cells
+    -> Steel.Effect.Atomic.SteelGhostT unit
+        opened
+        (star (pts_to p node_pcm (mk_node (some (Ghost.hide value)) (some (Ghost.hide next))))
+	  (pts_to_llist next l))
+        (fun _ ->
+            pts_to_llist p
+              (Ghost.hide (FStar.Pervasives.Native.Mktuple2 value next :: Ghost.reveal l)))
 
-let pts_to_llist_some p l =
-  match Ghost.reveal l with
-  | [] ->
-    change_equal_slprop (p `pts_to_llist` l) (p `pts_to_llist` []);
-    assert (p == nullptr);
-    assert (p =!= nullptr);
-    exfalso _ _ (fun res -> Ghost.reveal l == ((res.value, res.next) :: res.tl))
-  | (value, next) :: tl ->
-    change_equal_slprop (p `pts_to_llist` l) (p `pts_to_llist` ((value, next) :: tl));
-    {value; next; tl}
+assume val addr_of_value
+  (#value:Ghost.erased (option int))
+  (#next:Ghost.erased (option (Steel.C.Ptr.ptr node node)))
+  (p: Steel.C.Ptr.ptr node node)
+: Steel (Steel.C.Ptr.ptr node (option int))
+    (pts_to p node_pcm (mk_node value next))
+    (fun q ->
+       (pts_to p node_pcm (mk_node none next)) `star`
+       (pts_to q opt_pcm value))
+    (requires (fun _ -> True))
+    (ensures (fun _ q _ -> ptr_focused q p _value))
 
-val set_hd (p:ptr node node) (l:Ghost.erased cells) (value:int)
+assume val unaddr_of_value
+  (#value:Ghost.erased (option int))
+  (#next:Ghost.erased (option (Steel.C.Ptr.ptr node node)))
+  (p: Steel.C.Ptr.ptr node node)
+  (q: Steel.C.Ptr.ptr node (option int))
+: Steel unit
+    ((pts_to p node_pcm (mk_node none next)) `star`
+     (pts_to q opt_pcm value))
+    (fun q -> pts_to p node_pcm (mk_node value next))
+    (requires (fun _ -> ptr_focused q p _value))
+    (ensures (fun _ _ _ -> True))
+
+val set_first (p:ptr node) (l:Ghost.erased cells) (value:int)
 : SteelT unit
     (p `pts_to_llist` l)
     (fun _ -> p `pts_to_llist` cells_set_hd value l)
 
-// Problem: need (pts_to_or_null p pb v), where v =!= one, before can check whether it's null
-// Unclear how to rearrange pts_to_or_null
+val is_empty
+  (#l: Ghost.erased cells) (p: ptr node)
+: Steel bool
+    (p `pts_to_llist` l)
+    (fun _ -> p `pts_to_llist` l)
+    (requires fun _ -> True)
+    (ensures fun _ b _ -> b <==> p == nullptr)
+let is_empty #l p =
+  unfold_pts_to_llist p l;
+  let b = is_null p in
+  fold_pts_to_llist p l;
+  return b
 
-let set_hd p l new_value =
-  //let b = is_null p in
-  if true then begin
-    //pts_to_llist_nullptr p l;
-    sladmit(); return ()
+let set_first p l new_value =
+  let b = is_empty p in
+  if b then begin
+    pts_to_llist_nullptr p l;
+    return ()
   end else begin
-    sladmit(); return ()
-    //let res = pts_to_llist_some p l in
-    //let value: Ghost.erased int = Ghost.hide res.value in
-    //let next: Ghost.erased ptr = Ghost.hide res.next in
-    //let tl: Ghost.erased cells = Ghost.hide res.tl in
-    //change_equal_slprop (p `pts_to_llist` _) (p `pts_to_llist` _);
-    //let r' = elim_llist_cons p (Ghost.reveal value) (Ghost.reveal next) (Ghost.reveal tl) in
-    //let r: ref node node_pcm = r in
-    //change_equal_slprop
-    //  (Ghost.reveal r' `pts_to` mk_node (some value) (some next))
-    //  (r `pts_to` mk_node (some value) (some next));
-    //let r_value = addr_of_value r in
-    //r_value `opt_write` new_value;
-    //unaddr_of_value r r_value;
-    //intro_llist_cons r p new_value next tl;
-    //return ()
+    let res = elim_pts_to_llist_cons p l in
+    let p_value = addr_of_value p in
+    p_value `ptr_opt_write` new_value;
+    unaddr_of_value p p_value;
+    intro_pts_to_llist_cons' p new_value res.next res.tl;
+    return ()
   end
-
-// for the presentation, write write code for set_hd
-// based on assume val for needed selectors, then solve assumes
 
 let rec cells_set_nth (n:nat) (value:int) (l:cells) : Tot cells (decreases n) =
   if n = 0 then cells_set_hd value l
@@ -254,68 +352,98 @@ let rec cells_set_nth_nil n value
 = if n = 0 then () else cells_set_nth_nil (n - 1) value
 
 let llist_setter (n:nat) =
-  p:ptr node node -> l:Ghost.erased cells -> value:int ->
+  p:ptr node -> l:Ghost.erased cells -> value:int ->
   SteelT unit
     (p `pts_to_llist` l)
     (fun _ -> p `pts_to_llist` cells_set_nth n value l)
 
 let llist_set_zero: llist_setter 0 = set_hd
 
-(*
-let aux n (ih: llist_setter n) (p: ptr) (l: Ghost.erased cells) (new_value: int)
+// TODO set_hd: can make helper function is_empty to check whether list is empty or not
+
+let aux n value l = cells_set_nth (n + 1) value l
+
+let aux n (ih: llist_setter n) (p: ptr node) (l: Ghost.erased cells) (new_value: int)
 : SteelT unit
     (p `pts_to_llist` l)
     (fun _ -> p `pts_to_llist` cells_set_nth (n + 1) new_value l)
-= assume (Some? p);
-  // match p with
-  // | None ->
-  //   pts_to_llist_nullptr p l;
-  //   cells_set_nth_nil (n + 1) value;
-  //   change_equal_slprop
-  //     (None `pts_to_llist` [])
-  //     (p `pts_to_llist` cells_set_nth (n + 1) value l);
-  //   return ()
-  // | Some r ->
-  let Some r = p in
-    let res = pts_to_llist_some p l in
-    let value: Ghost.erased int = Ghost.hide res.value in
-    let next: Ghost.erased ptr = Ghost.hide res.next in
-    let tl: Ghost.erased cells = Ghost.hide res.tl in
-    //let value: Ghost.erased int = Ghost.hide (fst value_next_tl) in
-    //let next: Ghost.erased ptr = Ghost.hide (fst (snd value_next_tl)) in
-    //let tl: Ghost.erased cells = Ghost.hide (snd (snd value_next_tl)) in
-    change_equal_slprop (p `pts_to_llist` l)
-      (Some r `pts_to_llist`
-       Ghost.hide ((Ghost.reveal value, Ghost.reveal next) :: Ghost.reveal tl));
-    let r' = elim_llist_cons (Some r) (Ghost.reveal value) (Ghost.reveal next) (Ghost.reveal tl) in
-    let r: ref node node_pcm = r in
-    change_equal_slprop (Ghost.reveal r' `pts_to` mk_node (some value) (some next))
-      (r `pts_to` mk_node (some value) (some next));
+= unfold_pts_to_llist p l;
+  let b = is_null p in
+  fold_pts_to_llist p l;
+  assume (b == false);
+  //if b then begin
+  //  pts_to_llist_nullptr p l;
+  //  cells_set_nth_nil (n + 1) new_value;
+  //  return ()
+  //end else begin
+    let res = elim_pts_to_llist_cons p l in
+    let r = elim_pts_to p in
     let r_next = addr_of_next r in
-    let q: ptr = opt_read r_next in
-    assert (q == Ghost.reveal next);
+    let q = opt_read r_next in
     unaddr_of_next r r_next;
-    change_equal_slprop (Ghost.reveal next `pts_to_llist` _) (q `pts_to_llist` _);
-    ih q tl new_value;
-    change_equal_slprop (q `pts_to_llist` _) (Ghost.reveal next `pts_to_llist` _);
-    intro_llist_cons r (Ghost.reveal value) (Ghost.reveal next) _;
-//val intro_llist_cons
-//  (#opened:inames) (r: ref node node_pcm)
-//  (value: int) (next: ptr)
-//  (tl: cells)
-//: SteelGhostT unit opened
-//    ((r `pts_to` mk_node (some value) (some next)) `star` (next `pts_to_llist` tl))
-//    (fun _ -> Some r `pts_to_llist` ((value, next)::tl))
-    sladmit(); return ()
-    // //assert (Ghost.reveal r' == r);
-    // //slassert (Ghost.reveal r' `pts_to` mk_node (some value) (some next));
-    // let r_value = addr_of_value r in
-    // r_value `opt_write` new_value;
-    // unaddr_of_value r r_value;
-    // intro_llist_cons r new_value next tl;
-    // //change_equal_slprop (Ghost.reveal r' `pts_to` mk_node _ _) (r `pts_to` mk_node _ _);
-    // //sladmit(); return ()
-    // return ()
+    assert (q == res.next);
+    change_equal_slprop (res.next `pts_to_llist` _) (q `pts_to_llist` _);
+    ih q res.tl new_value;
+    //let p' = intro_pts_to r in
+    //change_equal_slprop (pts_to p' node_pcm _) (pts_to p node_pcm _);
+    //intro_pts_to_llist_cons p
+    //  (mk_node (some (Ghost.hide new_value)) (some (Ghost.hide res.next)))
+    //  new_value res.next res.tl;
+    sladmit();
+    return ()
+  //end
+
+  // assume (Some? p);
+  // // match p with
+  // // | None ->
+  // //   pts_to_llist_nullptr p l;
+  // //   cells_set_nth_nil (n + 1) value;
+  // //   change_equal_slprop
+  // //     (None `pts_to_llist` [])
+  // //     (p `pts_to_llist` cells_set_nth (n + 1) value l);
+  // //   return ()
+  // // | Some r ->
+  // let Some r = p in
+  //   let res = pts_to_llist_some p l in
+  //   let value: Ghost.erased int = Ghost.hide res.value in
+  //   let next: Ghost.erased ptr = Ghost.hide res.next in
+  //   let tl: Ghost.erased cells = Ghost.hide res.tl in
+  //   //let value: Ghost.erased int = Ghost.hide (fst value_next_tl) in
+  //   //let next: Ghost.erased ptr = Ghost.hide (fst (snd value_next_tl)) in
+  //   //let tl: Ghost.erased cells = Ghost.hide (snd (snd value_next_tl)) in
+  //   change_equal_slprop (p `pts_to_llist` l)
+  //     (Some r `pts_to_llist`
+  //      Ghost.hide ((Ghost.reveal value, Ghost.reveal next) :: Ghost.reveal tl));
+  //   let r' = elim_llist_cons (Some r) (Ghost.reveal value) (Ghost.reveal next) (Ghost.reveal tl) in
+  //   let r: ref node node_pcm = r in
+  //   change_equal_slprop (Ghost.reveal r' `pts_to` mk_node (some value) (some next))
+  //     (r `pts_to` mk_node (some value) (some next));
+  //   let r_next = addr_of_next r in
+  //   let q: ptr = opt_read r_next in
+  //   assert (q == Ghost.reveal next);
+  //   unaddr_of_next r r_next;
+  //   change_equal_slprop (Ghost.reveal next `pts_to_llist` _) (q `pts_to_llist` _);
+  //   ih q tl new_value;
+  //   change_equal_slprop (q `pts_to_llist` _) (Ghost.reveal next `pts_to_llist` _);
+  //   intro_llist_cons r (Ghost.reveal value) (Ghost.reveal next) _;
+//// val intro_llist_cons
+////   (#opened:inames) (r: ref node node_pcm)
+////   (value: int) (next: ptr)
+////   (tl: cells)
+//// : SteelGhostT unit opened
+////     ((r `pts_to` mk_node (some value) (some next)) `star` (next `pts_to_llist` tl))
+////     (fun _ -> Some r `pts_to_llist` ((value, next)::tl))
+  //   sladmit(); return ()
+  //   // //assert (Ghost.reveal r' == r);
+  //   // //slassert (Ghost.reveal r' `pts_to` mk_node (some value) (some next));
+  //   // let r_value = addr_of_value r in
+  //   // r_value `opt_write` new_value;
+  //   // unaddr_of_value r r_value;
+  //   // intro_llist_cons r new_value next tl;
+  //   // //change_equal_slprop (Ghost.reveal r' `pts_to` mk_node _ _) (r `pts_to` mk_node _ _);
+  //   // //sladmit(); return ()
+  //   // return ()
+  // let set_hd p l new_value =
 
 let llist_set_succ n (ih: llist_setter n): llist_setter (n + 1) =
   let aux (p: ptr) (l: Ghost.erased cells) (value: int)
@@ -362,8 +490,6 @@ let llist_set_succ n (ih: llist_setter n): llist_setter (n + 1) =
       // //sladmit(); return ()
       // return ()
   in aux
-
-*)
 
 // TODO look at #2319, construct module of (possibly null) pointers
 // (define pts_to_or_null; can compare against null only if points to non-unit)
